src/utils/Int.v
@@ -3,4 +3,3 @@ Require Export BinIntDef BinInt.
 Notation int := Z.
 
 Export Z.
-Open Scope Z_scope.
